Improvement of Coq appendix

Listings/SpecCert.v
@@ -7,45 +7,34 @@ Section SpecCert.
   | Hardware
     : Lh -> label.
 
-  Definition t :=
+  Definition model
+    : Type :=
     S -> label -> S -> Prop.
 
-  Definition _from
-             (tr:  S * label * S)
-    : S :=
-    match tr with (s, _, _) => s end.
-
-  Definition _to
-             (tr:  S * label * S)
-    : S :=
-    match tr with (_, _, s) => s end.
-
-  Definition _labelled
-             (tr:  S * label * S)
-    : label :=
-    match tr with (_, l, _) => l end.
-
-  Definition transition
-             (m:  t)
-    := { tr | m (_from tr) (_labelled tr) (_to tr) }.
-
   Definition from
-             {m:   t}
-             (tr:  transition m)
+             (tr:  S * label * S)
     : S :=
-    match tr with exist _ x _ => _from x end.
-
-  Definition labelled
-             {m:   t}
-             (tr:  transition m)
-    : label :=
-    match tr with exist _ x _ => _labelled x end.
+    fst (fst tr).
 
   Definition to
-             {m:   t}
-             (tr:  transition m)
+             (tr:  S * label * S)
     : S :=
-    match tr with exist _ x _ => _to x end.
+   snd tr.
+
+  Definition labelled
+             (tr:  S * label * S)
+    : label :=
+    snd (fst tr).
+
+  Definition transition
+             (m:  model)
+    : Type :=
+    { tr | m (from tr) (labelled tr) (to tr) }.
+
+  Notation "'[' x ']'" :=
+    (proj1_sig x).
+
+  Arguments exist [_ _] (_ _).
 
   Inductive sequence
             (a:  Type)
@@ -56,138 +45,131 @@ Section SpecCert.
           (rst:  sequence a)
     : sequence a.
 
-  Definition _init
-             {m:  t}
+  Arguments Ssingleton [a] (x).
+  Arguments Scons [a] (x rst).
+
+  Definition init
+             {m:  model}
              (seq:  sequence (transition m))
     : S :=
     match seq with
-    | Ssingleton _ tr
-      => from tr
-    | Scons _ tr _
-      => from tr
+    | Ssingleton tr
+      => from [tr]
+    | Scons tr _
+      => from [tr]
     end.
 
-  Fixpoint is_trace
-           {m:   t}
-           (tr:  sequence (transition m))
-    : Prop :=
-    match tr with
-    | Ssingleton _ _
-      => True
-    | Scons _ tr rst
-      => to tr = _init rst
-         /\ is_trace rst
-    end.
+  Inductive is_trace
+            {m:  model}
+    : sequence (transition m) -> Prop :=
+  | singleton_is_trace (tr:  transition m)
+    : is_trace (Ssingleton tr)
+  | step_is_trace (tr:   transition m)
+                  (rho:  sequence (transition m))
+                  (Heq:  to [tr] = init rho)
+                  (Hrec:  is_trace rho)
+    : is_trace (Scons tr rho).
 
   Definition trace
-             (m:  t) :=
+             (m:  model)
+    : Type :=
     { tr:  sequence (transition m) | is_trace tr }.
 
-  Definition init
-             {m:    t}
-             (rho:  trace m)
-    : S :=
-    _init (proj1_sig rho).
-
-  Fixpoint trans_aux
-           {m:    t}
+  Fixpoint trans
+           {m:    model}
            (rho:  sequence (transition m))
     : transition m -> Prop :=
     fun (tr:  transition m)
     => match rho with
-       | Ssingleton _ x
+       | Ssingleton x
          => tr = x
-       | Scons _ x rst
-         => tr = x \/ trans_aux rst tr
+       | Scons x rst
+         => tr = x \/ trans rst tr
        end.
 
-  Definition trans
-             {m:  t}
-             (rho:  trace m)
-    : transition m -> Prop :=
-    trans_aux (proj1_sig rho).
-
   Definition security_policy
-             (m:  t) :=
+             (m:  model) :=
     (trace m -> Prop) -> Prop.
 
   Definition security_property
-             (m:  t)
+             (m:  model)
              (prop:  trace m -> Prop)
     : security_policy m :=
     fun (traces:  trace m -> Prop)
     => forall (rho:  trace m), traces rho -> prop rho.
 
   Definition safety_property
-             {m:     t}
+             {m:     model}
              (prop:  transition m -> Prop) :=
     fun (traces:  trace m -> Prop)
     => forall (rho:  trace m),
         traces rho
         -> forall (tr: transition m),
-          trans rho tr
+          trans [rho] tr
           -> prop tr.
 
+  Definition if_software
+             (l:  label)
+             (P:  Ls -> Prop)
+    : Prop :=
+    match l with
+    | Software l
+      => P l
+    | Hardware _
+      => True
+    end.
+
   Record HSE
-         (m:  t) :=
-    { software:  Type
-      ; tcb:        software -> Prop
-      ; context:    S -> software
-      ; inv:        S -> Prop
-      ; behaviour:  S -> Ls -> Prop
-      ; law_1:      forall (tr:  transition m),
-          inv (from tr)
-          -> match (labelled tr) with
-             | Software l
-               => behaviour (from tr) l
-             | _
-               => True
-             end
-          -> inv (to tr)
-      ; law_2:      forall (tr:  transition m),
-          tcb (context (from tr))
-          -> match (labelled tr) with
-             | Software l
-               => behaviour (from tr) l
-             | _
-               => True
-             end
+         (m:  model) :=
+    { software:   Type
+    ; tcb:        software -> Prop
+    ; context:    S -> software
+    ; inv:        S -> Prop
+    ; behaviour:  S -> Ls -> Prop
+    ; law_1:      forall (tr:  transition m),
+        inv (from [tr])
+        -> if_software (labelled [tr])
+                       (behaviour (from [tr]))
+        -> inv (to [tr])
+    ; law_2:      forall (tr:  transition m),
+        tcb (context (from [tr]))
+        -> if_software (labelled [tr])
+                       (behaviour (from [tr]))
     }.
 
+  Arguments software [m] (_).
+  Arguments tcb [m] (_).
+  Arguments context [m] (_ _).
+  Arguments inv [m] (_ _).
+  Arguments behaviour [m] (_ _ _).
+
   Definition compliant_trace
-             {m:    t}
+             {m:    model}
              (hse:  HSE m)
              (rho:   trace m)
     : Prop :=
-    inv _ hse (init rho)
+    inv hse (init [rho])
     /\ forall (tr:  transition m),
-      trans rho tr
-      -> match (labelled tr) with
-         | Software l
-           => behaviour _ hse (from tr) l
-         | _
-           => True
-         end.
+      trans [rho] tr
+      -> if_software (labelled [tr])
+                     (behaviour hse (from [tr])).
 
   Lemma compliant_run_rec
-        {m:      t}
+        {m:      model}
         (hse:    HSE m)
         (x:      transition m)
         (rho:    sequence (transition m))
-        (Hcons:  is_trace (Scons (transition m) x rho))
+        (Hcons:  is_trace (Scons x rho))
         (Hrho:   is_trace rho)
-    : compliant_trace hse
-                      (exist _ (Scons (transition m) x rho)
-                             Hcons)
-      -> compliant_trace hse (exist _ rho Hrho).
+    : compliant_trace hse (exist (Scons x rho) Hcons)
+      -> compliant_trace hse (exist rho Hrho).
   Proof.
     intros Hcomp.
     inversion Hcomp as [Hinv Hbehaviour].
     constructor.
-    + inversion Hcons as [H0 Hrst].
-      unfold init.
+    + inversion Hcons; subst.
       cbn.
-      rewrite <- H0.
+      rewrite <- Heq.
       apply law_1.
       ++ apply Hinv.
       ++ apply Hbehaviour.
@@ -199,14 +181,14 @@ Section SpecCert.
   Qed.
 
   Lemma hse_inv_enforcement
-        {m:    t}
+        {m:    model}
         (hse:  HSE m)
     : forall (rho:  trace m),
       compliant_trace hse rho
       -> forall (tr:  transition m),
-        trans rho tr
-        -> inv _ hse (from tr)
-           /\ inv _ hse (to tr).
+        trans [rho] tr
+        -> inv hse (from [tr])
+           /\ inv hse (to [tr]).
   Proof.
     induction rho as [rho Hrho].
     induction rho.
@@ -238,34 +220,30 @@ Section SpecCert.
          exact Hinv.
          apply Hbehaviour.
          left; reflexivity.
-      ++ inversion Hrho as [Hs Hrst].
-         apply (IHrho Hrst).
+      ++ inversion Hrho; subst.
+         apply (IHrho Hrec).
          +++ eapply compliant_run_rec.
              apply Hcomp.
          +++ apply Htrans.
   Qed.
 
   Definition correct_hse
-             {m:    t}
+             {m:    model}
              (hse:  HSE m)
              (p:    security_policy m)
     : Prop :=
     p (compliant_trace hse) .
 
   Theorem safety_property_correct_hse
-          {m:    t}
+          {m:    model}
           (hse:  HSE m)
           (p:    transition m -> Prop)
     : (forall (rho:  trace m)
               (tr:   transition m),
-          trans rho tr
-          -> inv _ hse (from tr)
-          -> (match labelled tr with
-              | Software l
-                => behaviour _ hse (from tr) l
-              | _
-                => True
-              end)
+          trans [rho] tr
+          -> inv hse (from [tr])
+          -> if_software (labelled [tr])
+                         (behaviour hse (from [tr]))
           -> p tr)
       -> correct_hse hse (safety_property p).
   Proof.
@@ -279,4 +257,4 @@ Section SpecCert.
     + apply Hcomp.
       exact Htrans.
   Qed.
-  Section SpecCert.
+End SpecCert.
